Define 'endgame_wall_height'
Previously we were using hard-coded values for the wall height, but
that makes the code brittle and difficult to change if we need to make
the wall a different height. Now "endgame_wall_height" is opaque to
most of the endgame code.

Note that getting the wall height exactly right, and getting it to
match the wall height in the last 'make_run' block list has been
non-trivial. Fortunately, there is no problem using a larger wall, but
it must be done in such a way that we can prove a tight upper bound for
the size of the endgame blocked list. So if we trim some cells off the
top of the wall (as we were previously doing) the bound may be more
difficult to prove.

For now the wall height will be p(n + 2) + 2.

As an amusing aside: I can understand now why the original paper's
author just added an arbitrary 100 cells to the top of the wall!
It was as if to say, "Just assume it's tall enough!".

AngelDevil/Endgame.lean
@@ -39,19 +39,77 @@ structure Endgame (p : Nat) where
     exact Nat.add_one_pos _
   ))
 
-/- Produce the final 'blocked' list by taking the last blocked list
-   used in the endgame trace and removing any cells eaten by the devil
-   outside of the first quadrant or higher than the west wall.
+-- The west wall turned out to be taller than intended but any
+-- wall tall enough to keep the runner east of the y-axis will work.
+-- As long as we define the endgame blocked list to include the
+-- full height of the wall (above the x-axis) the final argument
+-- should still work.
+def endgame_wall_height {p : Nat} (E : Endgame p) : Nat := ((E.n + 2) * p) + 2
 
-   NOTE: It appears I actually used a later blocked list than I needed to as
-   the basis for endgame blocked list (see the proof of y-coordinate bounds
-   in 'endgame_west_of_wall' as an example). The result is that we have
-   a higher wall than we need and the Devil actually gets a couple free
-   moves at the end, but we've already proven this has no effect on the
-   endgame trace. Also, the extra wall calls will be trimmed anyway so
-   the final proof should be unaffected. -/
-abbrev endgame_blocked {p : Nat} (E : Endgame p) : List (Int × Int) :=
-  blocked_trim_quad1 (E.i + 1) run_start (make_block_list E.D p (E.n + 1)) (E.n * p + 1)
+-- The endgame wall has positive height
+lemma endgame_wall_height_pos {p : Nat} (E : Endgame p) :
+  0 < endgame_wall_height E := by
+  unfold endgame_wall_height
+  norm_num
+
+-- The endgame wall has non-zero height
+lemma endgame_wall_height_ge_one {p : Nat} (E : Endgame p) :
+  1 ≤ endgame_wall_height E := by
+  unfold endgame_wall_height
+  exact Nat.one_le_of_lt (Nat.add_one_pos _)
+
+-- The endgame trace never even touches the top cell of the wall
+lemma endgame_wall_height_lb {p : Nat} (E : Endgame p) :
+  E.n * p + 1 ≤ endgame_wall_height E - 1 := by
+  apply Nat.add_one_le_of_lt
+  unfold endgame_wall_height; simp
+  apply Nat.lt_add_one_of_le
+  rw [add_mul]
+  exact Nat.le_add_right _ _
+
+-- Produce the final 'blocked' list by taking the last blocked list
+-- used in the endgame trace and removing any cells eaten by the devil
+-- outside of the first quadrant or higher than the west wall.
+def endgame_blocked {p : Nat} (E : Endgame p) : List (Int × Int) :=
+  blocked_trim_quad1 (E.i + 1) run_start (make_block_list E.D p (E.n + 1))
+    (endgame_wall_height E - 1)
+
+-- Any cell with x = -1 and positive y-coordinate less than the
+-- height of the endgame wall will be in the endgame blocked list
+lemma endgame_blocked_mem_of_wall_mem {p : Nat} (E : Endgame p) :
+  ∀ i (_ : i < endgame_wall_height E),
+  (-1, (i : Int)) ∈ (endgame_blocked E) := by
+  intro i ilt
+  apply trace_trim_quad1_mem
+  · -- First, prove that the cell in question was in the wall to begin with
+    unfold make_block_list
+    apply List.mem_union_iff.mpr; right
+    rw [make_run_eaten_length]
+    -- Prove the y-coordinate bounds required to be in the west wall
+    apply west_wall_mem
+    · apply le_trans (Int.neg_ofNat_le_natCast _ 0)
+      exact Int.ofNat_le.mpr (Nat.zero_le _)
+    · unfold endgame_wall_height at ilt
+      rw [← one_add_one_eq_two, ← add_assoc] at ilt
+      convert Int.ofNat_le.mpr (Nat.le_of_lt_add_one ilt)
+  constructor
+  · simp
+  constructor
+  · simp
+    convert Int.ofNat_le.mpr (Nat.le_sub_one_of_lt ilt)
+    rw [Int.natCast_sub (endgame_wall_height_ge_one E)]
+    rw [Int.natCast_one]
+  constructor
+  · simp
+  use run_start
+  let BL' := make_block_list E.D p (E.n + 1)
+  constructor
+  · nth_rw 2 [← trace_getElem_zero_of_nonnil (E.i + 1) run_start BL']
+    · exact List.getElem_mem _
+    · apply List.ne_nil_of_length_pos
+      rw [trace_length]
+      exact Nat.add_one_pos _
+  · unfold run_start uvec_up loc; simp
 
 -- Prove that run_start is "valid" under the endgame blocked list
 lemma endgame_run_start_valid {p : Nat} (E : Endgame p) :
@@ -69,7 +127,9 @@ lemma endgame_run_start_valid {p : Nat} (E : Endgame p) :
     exact rsnmem
   · apply trace_trim_quad1_mem _ _ _ _ _ lormem
     unfold run_start left_of_runner uvec_up; simp
-    use (by rw [← Int.natCast_mul]; linarith), run_start
+    constructor
+    · exact endgame_wall_height_ge_one E
+    use run_start
     constructor
     · apply List.mem_of_getElem
       · convert trace_getElem_zero_of_nonnil _ _ _ hnnil
@@ -95,7 +155,7 @@ lemma endgame_trace_eq {p : Nat} (E : Endgame p) :
   have htrace := run_path_eq_trace_of_nice E.D p E.n (E.n + 1) (by simp) E.hnice
   have htake := trace_take RP.length run_start BL (E.i + 1) Eislt
   rw [htrace, ← htake]
-  apply trace_trim_quad1_unchanged (E.i + 1) run_start BL (E.n * p + 1)
+  apply trace_trim_quad1_unchanged (E.i + 1) run_start BL (endgame_wall_height E - 1)
   intro rs rsmem
   have rsmem' : rs ∈ RP := by
     unfold RP
@@ -111,9 +171,10 @@ lemma endgame_trace_eq {p : Nat} (E : Endgame p) :
   constructor
   · exact E.hynonneg rs rsmem''
   constructor
-  · apply Int.lt_add_one_of_le
-    rw [← Int.natCast_mul]
-    exact run_path_y_le E.D p E.n _ rsmem'
+  · rw [← Int.natCast_one, ← Int.natCast_sub (endgame_wall_height_ge_one E)]
+    apply lt_of_lt_of_le _ (Int.ofNat_le.mpr (endgame_wall_height_lb E))
+    rw [Int.natCast_add, Int.natCast_one]
+    exact Int.lt_add_one_of_le (run_path_y_le E.D p E.n rs rsmem')
   · exact E.hwest _ rsmem''
 
 def endgame_perimeter_length {p : Nat} (E : Endgame p) : Nat :=
@@ -369,7 +430,7 @@ lemma endgame_west_point_eq {p : Nat} (E : Endgame p) :
 -- Prove the coordinates and direction of all perimeter cells
 -- west of the wall.
 lemma endgame_west_of_wall {p : Nat} (E : Endgame p)
-  (i : Nat) (ilt : i < E.n * p + 2) :
+  (i : Nat) (ilt : i < endgame_wall_height E) :
   (endgame_perimeter E)[endgame_perimeter_length E - 2 - i]'(by
     rw [endgame_perimeter_length_def, ← Nat.sub_add_eq]
     apply Nat.sub_lt (endgame_perimeter_length_pos E)
@@ -383,8 +444,8 @@ lemma endgame_west_of_wall {p : Nat} (E : Endgame p)
     exact endgame_west_point_eq E
   rename' iz => inz; push_neg at inz
   have ipos : 0 < i := Nat.pos_of_ne_zero inz
-  have iplt : i - 1 < E.n * p + 1 := by
-    convert Nat.sub_lt_sub_right (Nat.one_le_of_lt ipos) ilt using 1
+  have iplt : i - 1 < endgame_wall_height E - 1 := by
+    exact Nat.sub_lt_sub_right (Nat.one_le_of_lt ipos) ilt
   have hvalid := endgame_run_start_valid E
   -- Use recursion to get the previous cell in the west wall
   -- (though we're working backward, so in some sense the "next" cell?)
@@ -426,36 +487,9 @@ lemma endgame_west_of_wall {p : Nat} (E : Endgame p)
   -- Prove that the cell at 'undo_left_turn' is always in the wall
   have huleft : loc (undo_turn_left { x := -2, y := ↑(i - 1), u := uvec_down }) ∈ BL := by
     unfold undo_turn_left uvec_down loc; simp
-    apply trace_trim_quad1_mem
-    · -- First, prove that the cell in question was in the wall to begin with
-      unfold make_block_list
-      apply List.mem_union_iff.mpr; right
-      rw [make_run_eaten_length]
-      -- Prove the y-coordinate bounds required to be in the west wall
-      apply west_wall_mem
-      · apply le_trans (Int.neg_ofNat_le_natCast _ 0)
-        rw [Int.ofNat_sub (Nat.one_le_of_lt ipos)]; simp
-      · apply Int.add_le_add_right (Int.ofNat_le.mpr _)
-        apply le_trans (Nat.le_of_lt_add_one iplt)
-        apply Nat.mul_le_mul_right
-        linarith
-    constructor
-    · simp; linarith
-    constructor
-    · simp
-      rw [← Int.natCast_mul]
-      exact Int.ofNat_le.mpr (Nat.le_of_lt_add_one iplt)
-    constructor
-    · simp
-    use run_start
-    let BL' := make_block_list E.D p (E.n + 1)
-    constructor
-    · nth_rw 2 [← trace_getElem_zero_of_nonnil (E.i + 1) run_start BL']
-      · exact List.getElem_mem _
-      · apply List.ne_nil_of_length_pos
-        rw [trace_length]
-        exact Nat.add_one_pos _
-    · unfold run_start uvec_up loc; simp
+    nth_rw 2 [← Int.natCast_one]
+    rw [← Int.natCast_add, Nat.sub_one_add_one inz]
+    exact endgame_blocked_mem_of_wall_mem E i ilt
   unfold undo_next_step; simp
   -- Prove that the cell at 'undo_move_forward' is *not* in the wall
   have huforward : loc (undo_move_forward { x := -2, y := ↑(i - 1), u := uvec_down }) ∉ BL := by
@@ -469,32 +503,37 @@ lemma endgame_west_of_wall {p : Nat} (E : Endgame p)
 -- Prove that the index of the north point is less than the
 -- length of the endgame perimeter
 lemma endgame_north_point_lt {p : Nat} (E : Endgame p) :
-  endgame_perimeter_length E - E.n * p - 4 < (endgame_perimeter E).length := by
+  endgame_perimeter_length E - endgame_wall_height E - 2 < (endgame_perimeter E).length := by
   rw [endgame_perimeter_length_def, ← Nat.sub_add_eq]
   exact Nat.sub_lt (endgame_perimeter_length_pos E) (by norm_num)
 
 -- Prove the coordinates and direction of the north point
 lemma endgame_north_point_eq {p : Nat} (E : Endgame p) :
-  (endgame_perimeter E)[endgame_perimeter_length E - E.n * p - 4]'(
-    endgame_north_point_lt E) = ⟨-1, E.n * p + 2, uvec_left⟩ := by
+  (endgame_perimeter E)[endgame_perimeter_length E - endgame_wall_height E - 2]'(
+    endgame_north_point_lt E) = ⟨-1, endgame_wall_height E, uvec_left⟩ := by
   let P := endgame_perimeter_length E
   let BL := endgame_blocked E
   have hvalid := endgame_run_start_valid E
   -- Save the details of the top perimeter cell west of the wall
-  have htw := endgame_west_of_wall E (E.n * p + 1) (Nat.lt_add_one _)
-  have hrw₀ : P - 2 - (E.n * p + 1) = P - 3 - E.n * p := by
-    rw [Nat.sub_add_eq, Nat.sub_right_comm, ← Nat.sub_add_eq _ 2]
+  have ewhpos : 0 < endgame_wall_height E := endgame_wall_height_pos E
+  have htw := endgame_west_of_wall E (endgame_wall_height E - 1) (Nat.sub_lt ewhpos (one_pos))
+  have hrw₀ : P - 2 - (endgame_wall_height E - 1) =
+              P - endgame_wall_height E - 1 := by
+    rw [Nat.sub_right_comm]
+    rw [Nat.sub_sub_right _ (endgame_wall_height_ge_one E)]
+    rw [← one_add_one_eq_two, Nat.sub_add_eq]
+    rw [Nat.sub_right_comm (P + 1), Nat.add_one_sub_one]
   rw [getElem_congr_idx hrw₀] at htw
-  have hpos : 0 < (P - 3 - E.n * p) := by
+  have hpos : 0 < (P - endgame_wall_height E - 1) := by
     apply Nat.pos_of_ne_zero
     contrapose! htw
     -- If 'htw' is true, the top-most perimeter cell west of the wall
     -- would be equal to 'run_start', which is obviously false.
     rw [getElem_congr_idx htw, endgame_perimeter_getElem_zero]
     unfold run_start uvec_up uvec_down; simp
-  have hlt : (P - 3 - E.n * p) < P := by
+  have hlt : (P - endgame_wall_height E - 1) < P := by
     rw [← Nat.sub_add_eq]
-    apply Nat.sub_lt (endgame_perimeter_length_pos E) (by norm_num)
+    exact Nat.sub_lt (endgame_perimeter_length_pos E) (by norm_num)
   -- Get the trace recurrence and apply 'undo_next_step' to both sides
   have htrace := trace_getElem_recurrence' P run_start BL _ hpos hlt
   apply congrArg (undo_next_step BL) at htrace
@@ -504,15 +543,18 @@ lemma endgame_north_point_eq {p : Nat} (E : Endgame p) :
   pick_goal 2; pick_goal 3
   · exact trace_wall_blocked_of_valid P run_start BL hvalid _ (List.getElem_mem _)
   · exact trace_avoids_blocked P run_start BL hvalid.1 _ (List.getElem_mem _)
-  have hrw₀ : P - E.n * p - 4 = P - 3 - E.n * p - 1 := by
-    rw [Nat.sub_right_comm _ 3, ← Nat.sub_add_eq _ 3 1]
-  rw [getElem_congr_idx hrw₀, ← htrace]
+  have hrw₁ : P - endgame_wall_height E - 2 = P - endgame_wall_height E - 1 -1 := by
+    rw [← one_add_one_eq_two, Nat.sub_add_eq]
+  rw [getElem_congr_idx hrw₁, ← htrace]
   unfold undo_next_step; simp
   -- Show that undoing a left turn starting at the top-most
   -- west-of-wall cell gives a cell that isn't in the wall
-  have huleft : loc (undo_turn_left { x := -2, y := ↑E.n * ↑p + 1, u := uvec_down }) ∉ BL := by
+  have huleft : loc (undo_turn_left { x := -2, y := ↑(endgame_wall_height E - 1), u := uvec_down }) ∉ BL := by
     apply trace_trim_quad1_notmem_of_lty
     unfold loc undo_turn_left uvec_down; simp
+    rw [Int.natCast_sub (endgame_wall_height_ge_one E)]
+    simp
   rw [if_neg huleft]
   unfold undo_turn_left uvec_down uvec_left; simp
-  rw [add_assoc, one_add_one_eq_two]
+  rw [← Int.natCast_one, ← Int.natCast_add, Nat.sub_one_add_one]
+  exact Nat.ne_zero_of_lt (endgame_wall_height_pos E)
